proofs/fstar/models/Alloc.Collections.Vec_deque.fsti
@@ -1,0 +1,75 @@
+module Alloc.Collections.Vec_deque
+#set-options "--fuel 0 --ifuel 1 --z3rlimit 15"
+open FStar.Mul
+open Rust_primitives
+
+// Overlay hax-lib 0.3.7's incomplete VecDeque model.  It omits the constructor
+// and update instance, and its index instance has an invalid unconditional
+// precondition.
+type t_VecDeque (v_T: Type0) (v_A: Type0) =
+  | VecDeque : Rust_primitives.Sequence.t_Seq v_T -> Core_models.Marker.t_PhantomData v_A
+    -> t_VecDeque v_T v_A
+
+let impl_4__new (#v_T: Type0) (_: Prims.unit) : t_VecDeque v_T Alloc.Alloc.t_Global =
+  VecDeque (Rust_primitives.Sequence.seq_empty #v_T ())
+    (Core_models.Marker.PhantomData <: Core_models.Marker.t_PhantomData Alloc.Alloc.t_Global)
+  <:
+  t_VecDeque v_T Alloc.Alloc.t_Global
+
+val impl_5__push_back (#v_T #v_A: Type0) (self: t_VecDeque v_T v_A) (x: v_T)
+    : Prims.Pure (t_VecDeque v_T v_A) Prims.l_True (fun _ -> Prims.l_True)
+
+val impl_5__len (#v_T #v_A: Type0) (self: t_VecDeque v_T v_A)
+    : Prims.Pure usize Prims.l_True (fun _ -> Prims.l_True)
+
+val impl_5__pop_front (#v_T #v_A: Type0) (self: t_VecDeque v_T v_A)
+    : Prims.Pure (t_VecDeque v_T v_A & Core_models.Option.t_Option v_T)
+      Prims.l_True
+      (fun _ -> Prims.l_True)
+
+// hax-lib 0.3.7 declares this precondition as true, but seq_index requires a
+// valid index.  Expose the actual bound to callers and to the implementation.
+[@@ FStar.Tactics.Typeclasses.tcinstance]
+let impl_6 (#v_T #v_A: Type0) : Core_models.Ops.Index.t_Index (t_VecDeque v_T v_A) usize =
+  {
+    f_Output = v_T;
+    f_index_pre =
+      (fun (self: t_VecDeque v_T v_A) (i: usize) ->
+        i <. Rust_primitives.Sequence.seq_len self._0);
+    f_index_post = (fun (self: t_VecDeque v_T v_A) (i: usize) (out: v_T) -> true);
+    f_index
+    =
+    fun (self: t_VecDeque v_T v_A) (i: usize) -> Rust_primitives.Sequence.seq_index #v_T self._0 i
+  }
+
+val update_at_index_default (#v_T #v_A: Type0)
+    (self: t_VecDeque v_T v_A) (i: usize) : v_T
+
+[@@ FStar.Tactics.Typeclasses.tcinstance]
+let update_at_index (#v_T #v_A: Type0)
+    : Core_models.Ops.Index.t_Index (t_VecDeque v_T v_A) usize =
+  {
+    f_Output = v_T;
+    f_index_pre = (fun _ _ -> true);
+    f_index_post = (fun _ _ _ -> true);
+    // Mutation expressions resolve indexing through this inherited instance.
+    // Totalize the out-of-bounds branch, while preserving real VecDeque reads
+    // whenever the source-level hax assumption holds.
+    f_index =
+      (fun (self: t_VecDeque v_T v_A) (i: usize) ->
+        if i <. Rust_primitives.Sequence.seq_len self._0
+        then Rust_primitives.Sequence.seq_index #v_T self._0 i
+        else update_at_index_default #v_T #v_A self i)
+  }
+
+[@@ FStar.Tactics.Typeclasses.tcinstance]
+let update_at_usize (#v_T #v_A: Type0)
+    : Rust_primitives.Hax.update_at_tc (t_VecDeque v_T v_A) usize =
+  {
+    super_index = update_at_index #v_T #v_A;
+    update_at =
+      (fun (self: t_VecDeque v_T v_A) (i: usize) (x: v_T) ->
+        if i <. Rust_primitives.Sequence.seq_len self._0
+        then VecDeque (FStar.Seq.upd self._0 (v i) x) self._1
+        else self)
+  }
