proofs/fstar/models/Alloc.Slice.fst
@@ -1,0 +1,37 @@
+module Alloc.Slice
+#set-options "--fuel 0 --ifuel 1 --z3rlimit 15"
+open FStar.Mul
+open Rust_primitives
+
+let impl__to_vec (#v_T: Type0) (s: t_Slice v_T) : Alloc.Vec.t_Vec v_T Alloc.Alloc.t_Global =
+  Alloc.Vec.Vec (Rust_primitives.Sequence.seq_from_slice #v_T s)
+    (Core_models.Marker.PhantomData <: Core_models.Marker.t_PhantomData Alloc.Alloc.t_Global)
+  <:
+  Alloc.Vec.t_Vec v_T Alloc.Alloc.t_Global
+
+let impl__into_vec (#v_T #v_A: Type0) (s: t_Slice v_T) : Alloc.Vec.t_Vec v_T v_A =
+  Alloc.Vec.Vec (Rust_primitives.Sequence.seq_from_slice #v_T s)
+    (Core_models.Marker.PhantomData <: Core_models.Marker.t_PhantomData v_A)
+  <:
+  Alloc.Vec.t_Vec v_T v_A
+
+// hax 0.3.7 still extracts slice `concat` calls using this identifier, but
+// removed it from the bundled F* model. Keep the opaque model from hax 0.3.6.
+assume
+val impl__concat (#v_T1 #v_T2: Type0) (s: t_Slice v_T1)
+  : Alloc.Vec.t_Vec v_T2 Alloc.Alloc.t_Global
+
+assume
+val impl__sort_by':
+    #v_T: Type0 ->
+    #v_F: Type0 ->
+    {| i0: Core_models.Ops.Function.t_Fn v_F (v_T & v_T) |} ->
+    s: t_Slice v_T ->
+    compare: v_F
+  -> t_Slice v_T
+
+unfold
+let impl__sort_by
+      (#v_T #v_F: Type0)
+      (#[FStar.Tactics.Typeclasses.tcresolve ()] i0: Core_models.Ops.Function.t_Fn v_F (v_T & v_T))
+     = impl__sort_by' #v_T #v_F #i0
