proofs/fstar/models/Spec.Utils.fsti
@@ -92,7 +92,11 @@ val v_XOF (v_LEN: usize{v v_LEN < pow2 32}) (input: t_Slice u8) : t_Array u8 v_L
 
 val update_at_range_lemma #n
   (s: t_Slice 't)
-  (i: Core_models.Ops.Range.t_Range (int_t n) {(Core_models.Ops.Range.impl_index_range_slice 't n).f_index_pre s i}) 
+  (i: Core_models.Ops.Range.t_Range (int_t n) {
+    v i.f_start >= 0 /\
+    v i.f_start <= v i.f_end /\
+    v i.f_end <= Seq.length s
+  })
   (x: t_Slice 't)
   : Lemma
     (requires (Seq.length x == v i.f_end - v i.f_start))
@@ -245,4 +249,3 @@ let inv_ntt_spec #len (vec_in: t_Array i16 len) (zeta: int) (i: nat{i < v len}) 
    ((v (Seq.index vec_in j) + v (Seq.index vec_in i)) % 3329)) /\
   ((v (Seq.index vec_out j) % 3329) ==
    (((v (Seq.index vec_in j) - v (Seq.index vec_in i)) * zeta * 169) % 3329))
-
